examples/Employee_DesignModel_UMLPart_generator_shallow.thy
@@ -63,8 +63,6 @@ Class Galaxy =
   attribute sound : unit
   attribute moving : bool
 
-Class.end OclAny
-
 Define_int [ 1000, 1200, 1300, 1800, 2600, 2900, 3200, 3500 ]
 
 Instance X\<^sub>P\<^sub>e\<^sub>r\<^sub>s\<^sub>o\<^sub>n1 :: Person = [ salary = 1300 , boss = X\<^sub>P\<^sub>e\<^sub>r\<^sub>s\<^sub>o\<^sub>n2 ]
